\renewcommand{\graphTensorSpacing}{1}

\[
\sum_{\substack{i_1,i_2,\cdots,i_n\\ \sum_{k=1}^{n}{i_k} =t}}
\left(
{t \choose {i_1,i_2,\cdots,i_n}}
\begin{tikzpicture}[baseline=-7ex]s
	\node[circle,draw=black!80,thick,fill=black,label=left:$A$] (AT) at (0,-2*\graphLineSpacing) {};
	\node[circle,draw=black!80,thick,fill=myGrey,label=above right:$(\Lambda_1)^{i_1}$] (X1) at (0 + 2*\graphLineSpacing,0) {};
	\draw[thick] (0 + 2*\graphLineSpacing - 0.2,0 + 0.2) -- (0 + 2*\graphLineSpacing + 0.2,0 - 0.2) {};
	\node[circle,draw=black!80,thick,fill=myGrey,label=above right:$(\Lambda_2)^{i_2}$] (X2) at (0 + 2*\graphLineSpacing,-2*\graphLineSpacing) {};
	\draw[thick] (0 + 2*\graphLineSpacing - 0.2,-2*\graphLineSpacing + 0.2) -- (0 + 2*\graphLineSpacing + 0.2,-2*\graphLineSpacing - 0.2) {};
	\node[circle,draw=black!80,thick,fill=myGrey,label=above right:$(\Lambda_n)^{i_n}$] (XN0) at (0 + 2*\graphLineSpacing,-5*\graphLineSpacing) {};
	\draw[thick] (0 + 2*\graphLineSpacing - 0.2,-5*\graphLineSpacing + 0.2) -- (0 + 2*\graphLineSpacing + 0.2,-5*\graphLineSpacing - 0.2) {};

	\node (n) at (0,-3.5*\graphLineSpacing){$n$};

	\draw[thick, draw=black] (AT) -- (0,0) -- (X1) -- (0 + 3*\graphLineSpacing,0) {};

	\draw[thick, draw=black] (AT) -- (X2) -- (0 + 3*\graphLineSpacing,-2*\graphLineSpacing) -- (0 + 3*\graphLineSpacing,-2*\graphLineSpacing) {};

	\draw[thick, draw=black] (AT) -- (0,-2.5*\graphLineSpacing) {}; 
	\draw[thick, dotted] (0,-2.5*\graphLineSpacing)  -- (n) -- (0,-4.5*\graphLineSpacing){};
	\draw[thick, draw=black] (0,-4.5*\graphLineSpacing) -- (0,-5*\graphLineSpacing) -- (0 + \graphLineSpacing,-5*\graphLineSpacing) -- (XN0)  -- (0 + 3*\graphLineSpacing,-5*\graphLineSpacing) {};
\end{tikzpicture}
\right)
\equiv
A
\circ
\left(
\sum_{k=1}^n
\begin{tikzpicture}[baseline=-7ex]s
	\node[circle,draw=black!80,thick,fill=black,label=left:$I$] (I) at (0,-2*\graphLineSpacing) {};
	\node[circle,draw=black!80,thick,fill=myGrey,label=above right:$\Lambda_{k}$] (X2) at (0 + 2*\graphLineSpacing,-2*\graphLineSpacing) {};
	\draw[thick] (0 + 2*\graphLineSpacing - 0.2,-2*\graphLineSpacing + 0.2) -- (0 + 2*\graphLineSpacing + 0.2,-2*\graphLineSpacing - 0.2) {};

	\node (n) at (0,-3.5*\graphLineSpacing){$n$};

	\draw[thick, draw=black] (AT) -- (0,0) --  (0 + 2*\graphLineSpacing,0) {};

	\draw[thick, draw=black, label=above:] (AT) -- node [above] {$k$} (X2) -- (0 + 3*\graphLineSpacing,-2*\graphLineSpacing) -- (0 + 3*\graphLineSpacing,-2*\graphLineSpacing) {};

	\draw[thick, draw=black] (AT) -- (0,-2.5*\graphLineSpacing) {}; 
	\draw[thick, dotted] (0,-2.5*\graphLineSpacing)  -- (n) -- (0,-4.5*\graphLineSpacing){};
	\draw[thick, draw=black] (0,-4.5*\graphLineSpacing) -- (0,-5*\graphLineSpacing) -- (0 + \graphLineSpacing,-5*\graphLineSpacing) -- (0 + 2*\graphLineSpacing,-5*\graphLineSpacing) {};
\end{tikzpicture}
\right)^{\circ t}
\] \\
\[ A
\circ
\left(
\sum_{k=1}^n
	\begin{tikzpicture}[baseline=-7ex]s
	\node[circle,draw=black!80,thick,fill=black,label=left:$I$] (I) at (0,-2*\graphLineSpacing) {};
	\node[circle,draw=black!80,thick,fill=myGrey,label=above right:$\Lambda_{k}$] (X2) at (0 + 2*\graphLineSpacing,-2*\graphLineSpacing) {};
	\draw[thick] (0 + 2*\graphLineSpacing - 0.2,-2*\graphLineSpacing + 0.2) -- (0 + 2*\graphLineSpacing + 0.2,-2*\graphLineSpacing - 0.2) {};

	\node (n) at (0,-3.5*\graphLineSpacing){$n$};

	\draw[thick, draw=black] (AT) -- (0,0) --  (0 + 2*\graphLineSpacing,0) {};

	\draw[thick, draw=black, label=above:] (AT) -- node [above] {$k$} (X2) -- (0 + 3*\graphLineSpacing,-2*\graphLineSpacing) -- (0 + 3*\graphLineSpacing,-2*\graphLineSpacing) {};

	\draw[thick, draw=black] (AT) -- (0,-2.5*\graphLineSpacing) {}; 
	\draw[thick, dotted] (0,-2.5*\graphLineSpacing)  -- (n) -- (0,-4.5*\graphLineSpacing){};
	\draw[thick, draw=black] (0,-4.5*\graphLineSpacing) -- (0,-5*\graphLineSpacing) -- (0 + \graphLineSpacing,-5*\graphLineSpacing) -- (0 + 2*\graphLineSpacing,-5*\graphLineSpacing) {};
\end{tikzpicture} \right)^{\circ t}_{i_1, i_2, \cdots, i_n}
\equiv A_{i_1, i_2, \cdots, i_n} \left( \sum_{k=1}^{n} {(\Lambda_k)}_{i_k,i_k} \right)^t\]

